Renaming in CakeML itree semantics

cakeml-semantics/cakeml_semanticsPropsScript.sml
@@ -32,24 +32,24 @@ Definition step_to_halt_cml_def:
     | SOME n => SOME $ step_n_cml n e
 End
 
-Definition dstep_n_cml_def:
-  dstep_n_cml env 0 d = d ∧
-  dstep_n_cml env (SUC n) (Dstep st) = dstep_n_cml env n (decl_step env st) ∧
-  dstep_n_cml env _ d = d
+Definition step_n_cml_def:
+  step_n_cml env 0 d = d ∧
+  step_n_cml env (SUC n) (Dstep st) = step_n_cml env n (decl_step env st) ∧
+  step_n_cml env _ d = d
 End
 
-Definition dis_halt_cml_def:
-  dis_halt_cml (Dstep step) = F ∧
-  dis_halt_cml (Dabort err) = T ∧
-  dis_halt_cml Ddone = T ∧
-  dis_halt_cml (Draise v) = T
+Definition is_halt_cml_def:
+  is_halt_cml (Dstep step) = F ∧
+  is_halt_cml (Dabort err) = T ∧
+  is_halt_cml Ddone = T ∧
+  is_halt_cml (Draise v) = T
 End
 
 Definition dstep_to_halt_cml_def:
   dstep_to_halt_cml env e =
-    case some n. dis_halt_cml (dstep_n_cml env n e) of
+    case some n. is_halt_cml (step_n_cml env n e) of
     | NONE => NONE
-    | SOME n => SOME $ dstep_n_cml env n e
+    | SOME n => SOME $ step_n_cml env n e
 End
 
 
@@ -183,17 +183,17 @@ val ditree_ss = simpLib.named_rewrites "ditree_ss" [
     dget_ffi_def
     ];
 
-Theorem dstep_n_same[simp]:
-  (∀env n. dstep_n env n Ddone = Ddone) ∧
-  (∀env n. dstep_n env n Dtype_error = Dtype_error) ∧
-  (∀env n st ev l p dcs.  dstep_n env n (Dffi st ev l p dcs) = Dffi st ev l p dcs) ∧
-  (∀env n v. dstep_n env n (Draise v) = Draise v) ∧
-  (∀env n. dstep_n_cml env n Ddone = Ddone) ∧
-  (∀env n err. dstep_n_cml env n (Dabort err) = (Dabort err)) ∧
-  (∀env n v. dstep_n_cml env n (Draise v) = Draise v)
+Theorem step_n_same[simp]:
+  (∀env n. step_n env n Ddone = Ddone) ∧
+  (∀env n. step_n env n Dtype_error = Dtype_error) ∧
+  (∀env n st ev l p dcs.  step_n env n (Dffi st ev l p dcs) = Dffi st ev l p dcs) ∧
+  (∀env n v. step_n env n (Draise v) = Draise v) ∧
+  (∀env n. step_n_cml env n Ddone = Ddone) ∧
+  (∀env n err. step_n_cml env n (Dabort err) = (Dabort err)) ∧
+  (∀env n v. step_n_cml env n (Draise v) = Draise v)
 Proof
   rpt conj_tac >> strip_tac >>
-  Cases >> rw[dstep_n_def, dstep_n_cml_def]
+  Cases >> rw[step_n_def, step_n_cml_def]
 QED
 
 Theorem is_Effi_def:
@@ -247,83 +247,83 @@ Proof
   every_case_tac >> gvs[application_not_Estuck]
 QED
 
-Theorem dstep_n_cml_eq_Dstep:
+Theorem step_n_cml_eq_Dstep:
   ∀env n e st.
-    dstep_n_cml env n e = Dstep st
-  ⇒ ∀m. m < n ⇒ ∃st'. dstep_n_cml env m e = Dstep st'
+    step_n_cml env n e = Dstep st
+  ⇒ ∀m. m < n ⇒ ∃st'. step_n_cml env m e = Dstep st'
 Proof
-  strip_tac >> Induct >> rw[dstep_n_cml_def] >>
-  Cases_on `e` >> gvs[dstep_n_cml_def] >>
-  Cases_on `m` >> gvs[dstep_n_cml_def]
+  strip_tac >> Induct >> rw[step_n_cml_def] >>
+  Cases_on `e` >> gvs[step_n_cml_def] >>
+  Cases_on `m` >> gvs[step_n_cml_def]
 QED
 
-Theorem dstep_n_cml_alt_def:
-  dstep_n_cml env 0 e = e ∧
-  dstep_n_cml env (SUC n) e = (
-    case dstep_n_cml env n e of
+Theorem step_n_cml_alt_def:
+  step_n_cml env 0 e = e ∧
+  step_n_cml env (SUC n) e = (
+    case step_n_cml env n e of
     | Dstep st => decl_step env st
     | e => e)
 Proof
-  rw[dstep_n_cml_def] >>
+  rw[step_n_cml_def] >>
   qid_spec_tac `e` >> qid_spec_tac `n` >>
-  Induct >> Cases >> rewrite_tac[dstep_n_cml_def] >> simp[]
+  Induct >> Cases >> rewrite_tac[step_n_cml_def] >> simp[]
 QED
 
-Theorem dstep_n_cml_add:
-  ∀env a b e. dstep_n_cml env (a + b) e = dstep_n_cml env a (dstep_n_cml env b e)
+Theorem step_n_cml_add:
+  ∀env a b e. step_n_cml env (a + b) e = step_n_cml env a (step_n_cml env b e)
 Proof
-  strip_tac >> Induct >> rw[dstep_n_cml_def] >>
-  simp[ADD_CLAUSES, dstep_n_cml_alt_def]
+  strip_tac >> Induct >> rw[step_n_cml_def] >>
+  simp[ADD_CLAUSES, step_n_cml_alt_def]
 QED
 
-Theorem dis_halt_cml_dstep_n_cml_eq:
+Theorem is_halt_cml_step_n_cml_eq:
   ∀n m e env.
-    dis_halt_cml (dstep_n_cml env n e) ∧
-    dis_halt_cml (dstep_n_cml env m e)
-  ⇒ dstep_n_cml env n e = dstep_n_cml env m e
+    is_halt_cml (step_n_cml env n e) ∧
+    is_halt_cml (step_n_cml env m e)
+  ⇒ step_n_cml env n e = step_n_cml env m e
 Proof
   rw[] >> wlog_tac `n < m` [`n`,`m`]
   >- (Cases_on `n = m` >> gvs[]) >>
   imp_res_tac LESS_STRONG_ADD >> gvs[] >>
-  gvs[dstep_n_cml_add |> ONCE_REWRITE_RULE[ADD_COMM]] >>
-  Cases_on `dstep_n_cml env n e` >> gvs[dis_halt_cml_def]
+  gvs[step_n_cml_add |> ONCE_REWRITE_RULE[ADD_COMM]] >>
+  Cases_on `step_n_cml env n e` >> gvs[is_halt_cml_def]
 QED
 
 
 (***** Results *****)
 
-Theorem decl_step_reln_eq_dstep_n_cml:
+Theorem decl_step_reln_eq_step_n_cml:
   (decl_step_reln env)^* st1 st2 ⇔
-  ∃n. dstep_n_cml env n (Dstep st1) = Dstep st2
+  ∃n. step_n_cml env n (Dstep st1) = Dstep st2
 Proof
   reverse $ eq_tac >> rw[] >> pop_assum mp_tac
   >- (
     map_every qid_spec_tac [`st2`,`st1`,`n`] >>
-    Induct >> rw[dstep_n_cml_alt_def] >>
+    Induct >> rw[step_n_cml_alt_def] >>
     every_case_tac >> gvs[] >>
     rw[Once relationTheory.RTC_CASES2] >> disj2_tac >>
     last_x_assum $ irule_at Any >> gvs[decl_step_reln_def]
     )
   >- (
     Induct_on `(decl_step_reln env)^*` >> rw[]
-    >- (qexists_tac `0` >> gvs[dstep_n_cml_def])
-    >- (qexists_tac `SUC n` >> gvs[dstep_n_cml_def, decl_step_reln_def])
+    >- (qexists_tac `0` >> gvs[step_n_cml_def])
+    >- (qexists_tac `SUC n` >> gvs[step_n_cml_def, decl_step_reln_def])
     )
 QED
 
-Theorem small_eval_dec_eq_dstep_n_cml:
+Theorem small_eval_dec_eq_step_n_cml:
   (small_eval_dec env dst (st, Rval e) ⇔
-    ∃n. dstep_n_cml env n (Dstep dst) = Dstep (st, Env e, [])) ∧
+    ∃n. step_n_cml env n (Dstep dst) = Dstep (st, Env e, [])) ∧
   (small_eval_dec env dst (st, Rerr (Rraise v)) ⇔
     ∃n dev dcs.
-      dstep_n_cml env n (Dstep dst) = Dstep (st, dev, dcs) ∧
+      step_n_cml env n (Dstep dst) = Dstep (st, dev, dcs) ∧
       decl_step env (st, dev, dcs) = Draise v) ∧
   (small_eval_dec env dst (st, Rerr (Rabort err)) ⇔
     ∃n dev dcs.
-      dstep_n_cml env n (Dstep dst) = Dstep (st, dev, dcs) ∧
+      step_n_cml env n (Dstep dst) = Dstep (st, dev, dcs) ∧
       decl_step env (st, dev, dcs) = Dabort err)
 Proof
-  rw[small_eval_dec_def, decl_step_reln_eq_dstep_n_cml] >>
+  rw[small_eval_dec_def, decl_step_reln_eq_step_n_cml] >>
   eq_tac >> rw[PULL_EXISTS] >> rpt $ goal_assum drule
 QED
 
@@ -331,19 +331,19 @@ Theorem dec_diverges_eq_step_to_halt_cml:
   small_decl_diverges env dst ⇔ dstep_to_halt_cml env (Dstep dst) = NONE
 Proof
   rw[dstep_to_halt_cml_def, small_decl_diverges_def,
-     decl_step_reln_eq_dstep_n_cml, PULL_EXISTS] >>
+     decl_step_reln_eq_step_n_cml, PULL_EXISTS] >>
   eq_tac >> rw[] >> gvs[e_step_reln_def]
   >- (
     DEEP_INTRO_TAC some_intro >> rw[] >>
-    Induct_on `x` >> rw[] >> gvs[dstep_n_cml_alt_def, dis_halt_cml_def] >>
+    Induct_on `x` >> rw[] >> gvs[step_n_cml_alt_def, is_halt_cml_def] >>
     CASE_TAC >> gvs[] >>
-    last_x_assum drule >> strip_tac >> gvs[decl_step_reln_def, dis_halt_cml_def]
+    last_x_assum drule >> strip_tac >> gvs[decl_step_reln_def, is_halt_cml_def]
     )
   >- (
     last_x_assum mp_tac >> DEEP_INTRO_TAC some_intro >> rw[] >>
     first_x_assum $ qspec_then `SUC n` assume_tac >>
-    gvs[dstep_n_cml_alt_def] >>
-    Cases_on `decl_step env b` >> gvs[dis_halt_cml_def, decl_step_reln_def]
+    gvs[step_n_cml_alt_def] >>
+    Cases_on `decl_step env b` >> gvs[is_halt_cml_def, decl_step_reln_def]
     )
 QED
 
@@ -377,70 +377,70 @@ QED
 
 (***** smallStep FFI-state lemmas *****)
 
-Theorem io_events_mono_dstep_n_cml:
+Theorem io_events_mono_step_n_cml:
   ∀env n dst1 dst2.
-    dstep_n_cml env n (Dstep dst1) = Dstep dst2
+    step_n_cml env n (Dstep dst1) = Dstep dst2
   ⇒ io_events_mono (FST dst1).ffi (FST dst2).ffi
 Proof
-  strip_tac >> Induct >> rw[dstep_n_cml_alt_def] >>
+  strip_tac >> Induct >> rw[step_n_cml_alt_def] >>
   irule io_events_mono_trans >>
   last_x_assum $ irule_at Any >>
-  qspecl_then [`env`,`SUC n`,`Dstep dst1`,`dst2`] mp_tac dstep_n_cml_eq_Dstep >>
-  gvs[dstep_n_cml_alt_def] >>
+  qspecl_then [`env`,`SUC n`,`Dstep dst1`,`dst2`] mp_tac step_n_cml_eq_Dstep >>
+  gvs[step_n_cml_alt_def] >>
   disch_then $ qspec_then `n` mp_tac >> gvs[] >> strip_tac >> gvs[] >>
   irule io_events_mono_decl_step >> simp[] >> goal_assum drule
 QED
 
-Theorem dstep_n_cml_preserved_FFI:
+Theorem step_n_cml_preserved_FFI:
   ∀n e e' env.
-    dstep_n_cml env n e = Dstep e' ∧ dget_ffi (Dstep e') = dget_ffi e
-  ⇒ ∀m. m < n ⇒ dget_ffi (dstep_n_cml env m e) = dget_ffi (Dstep e')
+    step_n_cml env n e = Dstep e' ∧ dget_ffi (Dstep e') = dget_ffi e
+  ⇒ ∀m. m < n ⇒ dget_ffi (step_n_cml env m e) = dget_ffi (Dstep e')
 Proof
   rw[] >> imp_res_tac LESS_STRONG_ADD >>
-  gvs[dstep_n_cml_add |> ONCE_REWRITE_RULE[ADD_COMM]] >> rename1 `SUC n` >>
-  Cases_on `dstep_n_cml env m e` >> gvs[] >>
+  gvs[step_n_cml_add |> ONCE_REWRITE_RULE[ADD_COMM]] >> rename1 `SUC n` >>
+  Cases_on `step_n_cml env m e` >> gvs[] >>
   PairCases_on `p` >> rename1 `(dst1,dev1,dcs1)` >>
   Cases_on `e` >> gvs[] >>
   PairCases_on `p` >> rename1 `_ = dget_ffi $ _ (dst,dev,dcs)` >>
   PairCases_on `e'` >>
-  rename1 `dstep_n_cml _ (SUC _) _ = Dstep (dst2,dev2,dcs2)` >>
-  imp_res_tac io_events_mono_dstep_n_cml >> gvs[dget_ffi_def] >>
+  rename1 `step_n_cml _ (SUC _) _ = Dstep (dst2,dev2,dcs2)` >>
+  imp_res_tac io_events_mono_step_n_cml >> gvs[dget_ffi_def] >>
   imp_res_tac io_events_mono_antisym >> gvs[]
 QED
 
 
 (***** itree-based lemmas *****)
 
-Theorem dstep_n_alt_def:
-  dstep_n env 0 e = e ∧
-  dstep_n env (SUC n) e = (
-    case dstep_n env n e of
+Theorem step_n_alt_def:
+  step_n env 0 e = e ∧
+  step_n env (SUC n) e = (
+    case step_n env n e of
     | Dstep dst dev dcs => dstep env dst dev dcs
     | e => e)
 Proof
-  rw[dstep_n_def] >>
+  rw[step_n_def] >>
   qid_spec_tac `e` >> qid_spec_tac `n` >>
-  Induct >> Cases >> rewrite_tac[dstep_n_def] >> simp[]
+  Induct >> Cases >> rewrite_tac[step_n_def] >> simp[]
 QED
 
-Theorem dstep_n_add:
-  ∀a b. dstep_n env (a + b) e = dstep_n env a (dstep_n env b e)
+Theorem step_n_add:
+  ∀a b. step_n env (a + b) e = step_n env a (step_n env b e)
 Proof
-  Induct >> rw[dstep_n_def] >>
-  simp[ADD_CLAUSES, dstep_n_alt_def]
+  Induct >> rw[step_n_def] >>
+  simp[ADD_CLAUSES, step_n_alt_def]
 QED
 
-Theorem dis_halt_dstep_n_eq:
+Theorem is_halt_step_n_eq:
   ∀n m env e.
-    dis_halt (dstep_n env n e) ∧
-    dis_halt (dstep_n env m e)
-  ⇒ dstep_n env n e = dstep_n env m e
+    is_halt (step_n env n e) ∧
+    is_halt (step_n env m e)
+  ⇒ step_n env n e = step_n env m e
 Proof
   rw[] >> wlog_tac `n < m` [`n`,`m`]
   >- (Cases_on `n = m` >> gvs[]) >>
   imp_res_tac LESS_STRONG_ADD >> gvs[] >>
-  gvs[dstep_n_add |> ONCE_REWRITE_RULE[ADD_COMM]] >>
-  Cases_on `dstep_n env n e` >> gvs[dis_halt_def, dstep_n_def]
+  gvs[step_n_add |> ONCE_REWRITE_RULE[ADD_COMM]] >>
+  Cases_on `step_n env n e` >> gvs[is_halt_def, step_n_def]
 QED
 
 Theorem application_thm:
@@ -548,50 +548,50 @@ Proof
   every_case_tac >> gvs[estep_to_Edone]
 QED
 
-Theorem dis_halt_dstep_n_const:
-  ∀n env e. dis_halt (dstep_n env n e) ⇒
-    ∀m. n < m ⇒ dstep_n env n e = dstep_n env m e
+Theorem is_halt_step_n_const:
+  ∀n env e. is_halt (step_n env n e) ⇒
+    ∀m. n < m ⇒ step_n env n e = step_n env m e
 Proof
-  Induct >> rw[dstep_n_def]
-  >- (Cases_on `e` >> gvs[dis_halt_def]) >>
-  Cases_on `e` >> gvs[dstep_n_def, dis_halt_def] >>
-  Cases_on `m` >> gvs[dstep_n_def]
+  Induct >> rw[step_n_def]
+  >- (Cases_on `e` >> gvs[is_halt_def]) >>
+  Cases_on `e` >> gvs[step_n_def, is_halt_def] >>
+  Cases_on `m` >> gvs[step_n_def]
 QED
 
-Theorem dis_halt_dstep_n_min:
-  ∀n env e. dis_halt (dstep_n env n e) ⇒
-  ∃m. m ≤ n ∧ dstep_n env m e = dstep_n env n e ∧
-      ∀l. l < m ⇒ ¬dis_halt (dstep_n env l e)
+Theorem is_halt_step_n_min:
+  ∀n env e. is_halt (step_n env n e) ⇒
+  ∃m. m ≤ n ∧ step_n env m e = step_n env n e ∧
+      ∀l. l < m ⇒ ¬is_halt (step_n env l e)
 Proof
-  Induct >> rw[dstep_n_alt_def] >>
-  every_case_tac >> gvs[dis_halt_def]
+  Induct >> rw[step_n_alt_def] >>
+  every_case_tac >> gvs[is_halt_def]
   >- (
     last_x_assum kall_tac >>
-    qexists_tac `SUC n` >> simp[dstep_n_alt_def] >> rw[] >>
+    qexists_tac `SUC n` >> simp[step_n_alt_def] >> rw[] >>
     CCONTR_TAC >> gvs[] >>
-    Cases_on `l' = n` >> gvs[dis_halt_def] >>
-    drule dis_halt_dstep_n_const >>
-    disch_then $ qspec_then `n` assume_tac >> gvs[dis_halt_def]
+    Cases_on `l' = n` >> gvs[is_halt_def] >>
+    drule is_halt_step_n_const >>
+    disch_then $ qspec_then `n` assume_tac >> gvs[is_halt_def]
     ) >>
-  last_x_assum $ qspecl_then [`env`,`e`] assume_tac >> gvs[dis_halt_def] >>
+  last_x_assum $ qspecl_then [`env`,`e`] assume_tac >> gvs[is_halt_def] >>
   qexists_tac `m` >> simp[]
 QED
 
-Theorem dstep_until_halt_take_step:
-  ∀dst dev dcs env. ¬ dis_halt (Dstep dst dev dcs)
-  ⇒ dstep_until_halt env (Dstep dst dev dcs) =
-    dstep_until_halt env (dstep env dst dev dcs)
+Theorem step_until_halt_take_step:
+  ∀dst dev dcs env. ¬ is_halt (Dstep dst dev dcs)
+  ⇒ step_until_halt env (Dstep dst dev dcs) =
+    step_until_halt env (dstep env dst dev dcs)
 Proof
-  rw[dstep_until_halt_def] >>
+  rw[step_until_halt_def] >>
   DEEP_INTRO_TAC some_intro >> rw[] >>
   DEEP_INTRO_TAC some_intro >> rw[]
   >- (
     qspecl_then [`x`,`SUC x'`,`env`,`Dstep dst dev dcs`]
-      assume_tac dis_halt_dstep_n_eq >>
-    gvs[dstep_n_def]
+      assume_tac is_halt_step_n_eq >>
+    gvs[step_n_def]
     )
-  >- (Cases_on `x` >> gvs[dstep_n_def])
-  >- (first_x_assum $ qspec_then `SUC x` assume_tac >> gvs[dstep_n_def])
+  >- (Cases_on `x` >> gvs[step_n_def])
+  >- (first_x_assum $ qspec_then `SUC x` assume_tac >> gvs[step_n_def])
 QED
 
 Theorem cml_io_unfold_err:
@@ -612,35 +612,35 @@ Proof
   PairCases_on `e` >> gvs[]
 QED
 
-Theorem dinterp:
-  dinterp env e =
-    case dstep_until_halt env e of
-    | DRet => Ret Termination
-    | DErr => Ret Error
-    | DDiv => Div
-    | DAct dst (s,ws1,ws2,n,env',cs) locs p dcs =>
+Theorem interp:
+  interp env e =
+    case step_until_halt env e of
+    | Ret => Ret Termination
+    | Err => Ret Error
+    | Div => Div
+    | Act dst (s,ws1,ws2,n,env',cs) locs p dcs =>
         Vis (s, ws1, ws2)
           (λa. case a of
                 | INL x => Ret $ FinalFFI (s, ws1, ws2) x
                 | INR y =>
                     if LENGTH ws2 = LENGTH y then
-                      dinterp env $
+                      interp env $
                         Dstep (dst with refs := LUPDATE (W8array y) n dst.refs)
                           (ExpVal env' (Val $ Conv NONE []) cs locs p) dcs
                     else Ret $ FinalFFI (s, ws1, ws2) FFI_failed)
 Proof
-  rw[dinterp_def] >> rw[Once cml_io_unfold_err] >> simp[] >>
+  rw[interp_def] >> rw[Once cml_io_unfold_err] >> simp[] >>
   CASE_TAC >> gvs[] >> rw[FUN_EQ_THM] >> PairCases_on `p` >> gvs[]
 QED
 
-Theorem trace_prefix_dinterp:
-  trace_prefix 0 (oracle, ffi_st) (dinterp env e) = ([], NONE) ∧
-  trace_prefix (SUC n) (oracle, ffi_st) (dinterp env e) =
-    case dstep_until_halt env e of
-    | DRet => ([], SOME Termination)
-    | DErr => ([], SOME Error)
-    | DDiv => ([], NONE)
-    | DAct dst (s,conf,ws,lnum,env',cs) locs pat dcs =>
+Theorem trace_prefix_interp:
+  trace_prefix 0 (oracle, ffi_st) (interp env e) = ([], NONE) ∧
+  trace_prefix (SUC n) (oracle, ffi_st) (interp env e) =
+    case step_until_halt env e of
+    | Ret => ([], SOME Termination)
+    | Err => ([], SOME Error)
+    | Div => ([], NONE)
+    | Act dst (s,conf,ws,lnum,env',cs) locs pat dcs =>
         case oracle s ffi_st conf ws of
         | Oracle_return ffi_st' ws' =>
             if LENGTH ws ≠ LENGTH ws' ∧ n = 0 then
@@ -649,7 +649,7 @@ Theorem trace_prefix_dinterp:
               ([], SOME $ FinalFFI (s, conf, ws) FFI_failed)
             else let (io, res) =
               trace_prefix n (oracle, ffi_st')
-                (dinterp env $
+                (interp env $
                   Dstep (dst with refs := LUPDATE (W8array ws') lnum dst.refs)
                     (ExpVal env' (Val $ Conv NONE []) cs locs pat) dcs)
             in ((IO_event s conf (ZIP (ws,ws')))::io, res)
@@ -657,7 +657,7 @@ Theorem trace_prefix_dinterp:
             if n = 0 then ([], NONE) else
             ([], SOME $ FinalFFI (s, conf, ws) outcome)
 Proof
-  rw[trace_prefix_def] >> rw[Once dinterp] >>
+  rw[trace_prefix_def] >> rw[Once interp] >>
   CASE_TAC >> gvs[trace_prefix_def] >>
   PairCases_on `p` >> gvs[trace_prefix_def] >>
   reverse $ CASE_TAC >> gvs[]
